Rename Step to ArStep and StepStar to ArStepStar and add boolean expressions with evaluation function

ExprEval/Basic.lean
@@ -1,5 +1,7 @@
 variable (V: Type)
 
+-- Arithmetic Expressions
+
 inductive ArExpr: Type
     | Const: Int -> ArExpr
     | Add: ArExpr -> ArExpr -> ArExpr
@@ -18,43 +20,43 @@ def eval (val: V -> Int) (e: ArExpr V) : Int :=
 
 -- My small steps semantic
 
-inductive Step: (val: V -> Int) -> (ArExpr V) -> (ArExpr V) -> Prop where
+inductive ArStep: (val: V -> Int) -> (ArExpr V) -> (ArExpr V) -> Prop where
     | getVarValue (var: V) :
-        Step
+        ArStep
             val
             (ArExpr.Var var)
             (ArExpr.Const (val var))
     | addConstConst(n1 n2: Int) :
-        Step
+        ArStep
             val
             (ArExpr.Add (ArExpr.Const n1) (ArExpr.Const n2))
             (ArExpr.Const (n1 + n2))
     | subConstConst(n1 n2: Int) :
-        Step
+        ArStep
             val
             (ArExpr.Sub (ArExpr.Const n1) (ArExpr.Const n2))
             (ArExpr.Const (n1 - n2))
     | mulConstConst(n1 n2: Int) :
-        Step
+        ArStep
             val
             (ArExpr.Mul (ArExpr.Const n1) (ArExpr.Const n2))
             (ArExpr.Const (n1 * n2))
-    | addLeft (e1 e1' e2) : Step val e1 e1' -> Step val (ArExpr.Add e1 e2) (ArExpr.Add e1' e2)
+    | addLeft (e1 e1' e2) : ArStep val e1 e1' -> ArStep val (ArExpr.Add e1 e2) (ArExpr.Add e1' e2)
 
-    | subLeft (e1 e1' e2) : Step val e1 e1' -> Step val (ArExpr.Sub e1 e2) (ArExpr.Sub e1' e2)
+    | subLeft (e1 e1' e2) : ArStep val e1 e1' -> ArStep val (ArExpr.Sub e1 e2) (ArExpr.Sub e1' e2)
 
-    | mulLeft (e1 e1' e2) : Step val e1 e1' -> Step val (ArExpr.Mul e1 e2) (ArExpr.Mul e1' e2)
+    | mulLeft (e1 e1' e2) : ArStep val e1 e1' -> ArStep val (ArExpr.Mul e1 e2) (ArExpr.Mul e1' e2)
 
-    | addRight (n: Int) (e2 e2': ArExpr V) : Step val e2 e2' -> Step val (ArExpr.Add (ArExpr.Const n) e2)  (ArExpr.Add (ArExpr.Const n) e2')
+    | addRight (n: Int) (e2 e2': ArExpr V) : ArStep val e2 e2' -> ArStep val (ArExpr.Add (ArExpr.Const n) e2)  (ArExpr.Add (ArExpr.Const n) e2')
 
-    | subRight (n: Int) (e2 e2': ArExpr V) : Step val e2 e2' -> Step val (ArExpr.Sub (ArExpr.Const n) e2)  (ArExpr.Sub (ArExpr.Const n) e2')
-    | mulRight (n: Int) (e2 e2': ArExpr V) : Step val e2 e2' -> Step val (ArExpr.Mul (ArExpr.Const n) e2)  (ArExpr.Mul (ArExpr.Const n) e2')
+    | subRight (n: Int) (e2 e2': ArExpr V) : ArStep val e2 e2' -> ArStep val (ArExpr.Sub (ArExpr.Const n) e2)  (ArExpr.Sub (ArExpr.Const n) e2')
+    | mulRight (n: Int) (e2 e2': ArExpr V) : ArStep val e2 e2' -> ArStep val (ArExpr.Mul (ArExpr.Const n) e2)  (ArExpr.Mul (ArExpr.Const n) e2')
 
-inductive StepStar : (val: V -> Int) -> (ArExpr V) -> (ArExpr V) -> Prop where
-    | refl val e : StepStar val e e
-    | trans e₁ e₂ e₃ : (Step V val) e₁ e₂ -> StepStar val e₂ e₃ -> StepStar val e₁ e₃
+inductive ArStepStar : (val: V -> Int) -> (ArExpr V) -> (ArExpr V) -> Prop where
+    | refl val e : ArStepStar val e e
+    | trans e₁ e₂ e₃ : (ArStep V val) e₁ e₂ -> ArStepStar val e₂ e₃ -> ArStepStar val e₁ e₃
 
-theorem step_preserve_eval (e e': ArExpr V): (Step V val) e e' -> eval V val e = eval V val e' := by
+theorem arstep_preserve_eval (e e': ArExpr V): (ArStep V val) e e' -> eval V val e = eval V val e' := by
     intro h
     induction h with
 
@@ -73,145 +75,169 @@ theorem step_preserve_eval (e e': ArExpr V): (Step V val) e e' -> eval V val e =
     | getVarValue var => simp [eval]
 
 
-theorem stepstar_preserves_eval (e e': ArExpr V) :
-    StepStar V val e e' -> eval V val e = eval V val e' := by
+theorem arstepstar_preserves_eval (e e': ArExpr V) :
+    ArStepStar V val e e' -> eval V val e = eval V val e' := by
     intro h
     induction h with
     | refl _ => rfl
-    | trans _ _ _ h1 _ ih => rw [step_preserve_eval _ _ _ h1, ih]
+    | trans _ _ _ h1 _ ih => rw [arstep_preserve_eval _ _ _ h1, ih]
 
-theorem soundness (e: ArExpr V) (v: Int) :
-    StepStar V val e (ArExpr.Const v) -> eval V val e = v := by
-    exact stepstar_preserves_eval _ _ _
-
-theorem stepstar_add_left (e1 e1' e2: ArExpr V) :
-    StepStar V val e1 e1' -> StepStar V val (ArExpr.Add e1 e2) (ArExpr.Add e1' e2) := by
+theorem arstepstar_add_left (e1 e1' e2: ArExpr V) :
+    ArStepStar V val e1 e1' -> ArStepStar V val (ArExpr.Add e1 e2) (ArExpr.Add e1' e2) := by
     intro h
     induction h with
-    | refl _ => apply StepStar.refl
+    | refl _ => apply ArStepStar.refl
     | trans _ _ _ step _ ih =>
-        apply StepStar.trans
-        . exact Step.addLeft _ _ _ step
+        apply ArStepStar.trans
+        . exact ArStep.addLeft _ _ _ step
         . exact ih
 
-theorem stepstar_add_right (n: Int) (e2 e2': ArExpr V) :
-    StepStar V val e2 e2' ->
-        StepStar V val
+theorem arstepstar_add_right (n: Int) (e2 e2': ArExpr V) :
+    ArStepStar V val e2 e2' ->
+        ArStepStar V val
             (ArExpr.Add (ArExpr.Const n) e2)
             (ArExpr.Add (ArExpr.Const n) e2') := by
     intro h
     induction h with
-    | refl _ => apply StepStar.refl
+    | refl _ => apply ArStepStar.refl
     | trans e1 e2 e3 step1 step2 ih =>
-        apply StepStar.trans
-        . apply Step.addRight _ _ _ step1
+        apply ArStepStar.trans
+        . apply ArStep.addRight _ _ _ step1
         . exact ih
 
 
 
-theorem stepstar_sub_left (e1 e1' e2: ArExpr V) :
-    StepStar V val e1 e1' ->
-        StepStar V val
+theorem arstepstar_sub_left (e1 e1' e2: ArExpr V) :
+    ArStepStar V val e1 e1' ->
+        ArStepStar V val
             (ArExpr.Sub e1 e2)
             (ArExpr.Sub e1' e2) := by
     intro h
     induction h with
-    | refl _ => apply StepStar.refl
+    | refl _ => apply ArStepStar.refl
     | trans _ _ _ step _ ih =>
-        apply StepStar.trans
-        . exact Step.subLeft _ _ _ step
+        apply ArStepStar.trans
+        . exact ArStep.subLeft _ _ _ step
         . exact ih
 
-theorem stepstar_sub_right (n: Int) (e2 e2': ArExpr V) :
-    StepStar V val e2 e2' ->
-        StepStar V val
+theorem arstepstar_sub_right (n: Int) (e2 e2': ArExpr V) :
+    ArStepStar V val e2 e2' ->
+        ArStepStar V val
             (ArExpr.Sub (ArExpr.Const n) e2)
             (ArExpr.Sub (ArExpr.Const n) e2') := by
     intro h
     induction h with
-    | refl _ => apply StepStar.refl
+    | refl _ => apply ArStepStar.refl
     | trans e1 e2 e3 step1 step2 ih =>
-        apply StepStar.trans
-        . apply Step.subRight _ _ _ step1
+        apply ArStepStar.trans
+        . apply ArStep.subRight _ _ _ step1
         . exact ih
 
 
 
-theorem stepstar_mul_left (e1 e1' e2: ArExpr V) :
-    StepStar V val e1 e1' ->
-        StepStar V val
+theorem arstepstar_mul_left (e1 e1' e2: ArExpr V) :
+    ArStepStar V val e1 e1' ->
+        ArStepStar V val
             (ArExpr.Mul e1 e2)
             (ArExpr.Mul e1' e2) := by
     intro h
     induction h with
-    | refl _ => apply StepStar.refl
+    | refl _ => apply ArStepStar.refl
     | trans _ _ _ step _ ih =>
-        apply StepStar.trans
-        . exact Step.mulLeft _ _ _ step
+        apply ArStepStar.trans
+        . exact ArStep.mulLeft _ _ _ step
         . exact ih
 
-theorem stepstar_mul_right (n: Int) (e2 e2': ArExpr V) :
-    StepStar V val e2 e2' ->
-        StepStar V val
+theorem arstepstar_mul_right (n: Int) (e2 e2': ArExpr V) :
+    ArStepStar V val e2 e2' ->
+        ArStepStar V val
             (ArExpr.Mul (ArExpr.Const n) e2)
             (ArExpr.Mul (ArExpr.Const n) e2') := by
     intro h
     induction h with
-    | refl _ => apply StepStar.refl
+    | refl _ => apply ArStepStar.refl
     | trans e1 e2 e3 step1 step2 ih =>
-        apply StepStar.trans
-        . apply Step.mulRight _ _ _ step1
+        apply ArStepStar.trans
+        . apply ArStep.mulRight _ _ _ step1
         . exact ih
 
 theorem chasles_step_star {e1 e2 e3: ArExpr V}:
-    StepStar V val e1 e2 ->
-        StepStar V val e2 e3 ->
-            StepStar V val e1 e3 := by
+    ArStepStar V val e1 e2 ->
+        ArStepStar V val e2 e3 ->
+            ArStepStar V val e1 e3 := by
     intros h1 h2
     induction h1 with
     | refl e => exact h2
     | trans a b c step rest ihn =>
         have h3 := ihn h2
-        have h4 := StepStar.trans _ _ _ step h3
+        have h4 := ArStepStar.trans _ _ _ step h3
         exact h4
 
-theorem completeness (e: ArExpr V) : StepStar V val e (ArExpr.Const (eval V val e)) := by
+
+theorem eval_soundness (e: ArExpr V) (v: Int) :
+    ArStepStar V val e (ArExpr.Const v) -> eval V val e = v := by
+    exact arstepstar_preserves_eval _ _ _
+
+
+theorem eval_completeness (e: ArExpr V) : ArStepStar V val e (ArExpr.Const (eval V val e)) := by
     induction e with
     | Const x =>
         simp [eval]
-        exact StepStar.refl _ _
+        exact ArStepStar.refl _ _
     | Add e1 e2 ih1 ih2 =>
-        -- ih1 : StepStar e1 (ArExpr.Const (eval e1))
-        -- ih2 : StepStar e2 (ArExpr.Const (eval e2))
+        -- ih1 : ArStepStar e1 (ArExpr.Const (eval e1))
+        -- ih2 : ArStepStar e2 (ArExpr.Const (eval e2))
         simp [eval]
-        have a := stepstar_add_left _ _ _ e2 ih1
-        have b := stepstar_add_right _ (eval V val e1) e2 _ ih2
-        have c := Step.addConstConst (val := val) (eval V val e1) (eval V val e2)
-        have d := StepStar.trans _ _ _ c (StepStar.refl _ (ArExpr.Const (eval V val e1 + eval V val e2)))
+        have a := arstepstar_add_left _ _ _ e2 ih1
+        have b := arstepstar_add_right _ (eval V val e1) e2 _ ih2
+        have c := ArStep.addConstConst (val := val) (eval V val e1) (eval V val e2)
+        have d := ArStepStar.trans _ _ _ c (ArStepStar.refl _ (ArExpr.Const (eval V val e1 + eval V val e2)))
         have e := chasles_step_star _ a (chasles_step_star _ b d)
         exact e
     | Sub e1 e2 ih1 ih2 =>
-        -- ih1 : StepStar e1 (ArExpr.Const (eval e1))
-        -- ih2 : StepStar e2 (ArExpr.Const (eval e2))
+        -- ih1 : ArStepStar e1 (ArExpr.Const (eval e1))
+        -- ih2 : ArStepStar e2 (ArExpr.Const (eval e2))
         simp [eval]
-        have a := stepstar_sub_left _ _ _ e2 ih1
-        have b := stepstar_sub_right _ (eval V val e1) e2 _ ih2
-        have c := Step.subConstConst (val := val) (eval V val e1) (eval V val e2)
-        have d := StepStar.trans _ _ _ c (StepStar.refl _ (ArExpr.Const  (eval V val e1 - eval V val e2)))
+        have a := arstepstar_sub_left _ _ _ e2 ih1
+        have b := arstepstar_sub_right _ (eval V val e1) e2 _ ih2
+        have c := ArStep.subConstConst (val := val) (eval V val e1) (eval V val e2)
+        have d := ArStepStar.trans _ _ _ c (ArStepStar.refl _ (ArExpr.Const  (eval V val e1 - eval V val e2)))
         have e := chasles_step_star _ a (chasles_step_star _ b d)
         exact e
     | Mul e1 e2 ih1 ih2 =>
-        -- ih1 : StepStar e1 (ArExpr.Const (eval e1))
-        -- ih2 : StepStar e2 (ArExpr.Const (eval e2))
+        -- ih1 : ArStepStar e1 (ArExpr.Const (eval e1))
+        -- ih2 : ArStepStar e2 (ArExpr.Const (eval e2))
         simp [eval]
-        have a := stepstar_mul_left _ _ _ e2 ih1
-        have b := stepstar_mul_right _ (eval V val e1) e2 _ ih2
-        have c := Step.mulConstConst (val := val) (eval V val e1) (eval V val e2)
-        have d := StepStar.trans _ _ _ c (StepStar.refl _ (ArExpr.Const (eval  V val e1 * eval V val e2)))
+        have a := arstepstar_mul_left _ _ _ e2 ih1
+        have b := arstepstar_mul_right _ (eval V val e1) e2 _ ih2
+        have c := ArStep.mulConstConst (val := val) (eval V val e1) (eval V val e2)
+        have d := ArStepStar.trans _ _ _ c (ArStepStar.refl _ (ArExpr.Const (eval  V val e1 * eval V val e2)))
         have e := chasles_step_star _ a (chasles_step_star _ b d)
         exact e
     | Var var =>
         simp [eval]
-        have a := Step.getVarValue var (val := val)
-        have b := StepStar.refl val (ArExpr.Const (val var))
-        exact StepStar.trans (val := val) _ _ _ a b
+        have a := ArStep.getVarValue var (val := val)
+        have b := ArStepStar.refl val (ArExpr.Const (val var))
+        exact ArStepStar.trans (val := val) _ _ _ a b
+
+
+-- Boolean Expressions
+
+inductive BoolExpr : Type
+    | True: BoolExpr
+    | False : BoolExpr
+    | Less: ArExpr V -> ArExpr V -> BoolExpr
+    | Eq: ArExpr V -> ArExpr V -> BoolExpr
+    | Not : BoolExpr -> BoolExpr
+    | And : BoolExpr -> BoolExpr -> BoolExpr
+    | Or : BoolExpr -> BoolExpr -> BoolExpr
+
+def eval_bool (val: V -> Int) (e: BoolExpr V): Bool :=
+    match e with
+    | BoolExpr.True => true
+    | BoolExpr.False => false
+    | BoolExpr.Less l r =>  (eval V val l) < (eval V val r)
+    | BoolExpr.Eq l r => (eval V val l) == (eval V val r)
+    | BoolExpr.Not e => not (eval_bool val e)
+    | BoolExpr.And l r => if eval_bool val l then eval_bool val r else false
+    | BoolExpr.Or l r => if eval_bool val l then true else eval_bool val r
